Working on implementing Extmap with gmap
First few functions done, have compiling OCaml code with extraction

src/util/Extmap.v
@@ -3,6 +3,130 @@
   instead of balanced binary trees*)
 From stdpp Require Import gmap.  
 
+(*Let's see*)
+(*
+Section MoreUnion.
+
+Local Open Scope positive_scope.
+
+Local Notation "P ~ 0" := (λ p, P p~0) : function_scope.
+Local Notation "P ~ 1" := (λ p, P p~1) : function_scope.
+
+(*JOSH - smart constructor - exposes interface of left, node, right,
+  produces actual term*)
+Local Definition GNode {A P}
+    (ml : gmap_dep A P~0)
+    (mx : option (P 1 * A)) (mr : gmap_dep A P~1) : gmap_dep A P :=
+  match ml, mx, mr with
+  | GEmpty, None, GEmpty => GEmpty
+  | GEmpty, None, GNodes r => GNodes (GNode001 r)
+  | GEmpty, Some (p,x), GEmpty => GNodes (GNode010 p x)
+  | GEmpty, Some (p,x), GNodes r => GNodes (GNode011 p x r)
+  | GNodes l, None, GEmpty => GNodes (GNode100 l)
+  | GNodes l, None, GNodes r => GNodes (GNode101 l r)
+  | GNodes l, Some (p,x), GEmpty => GNodes (GNode110 l p x)
+  | GNodes l, Some (p,x), GNodes r => GNodes (GNode111 l p x r)
+  end.
+
+(*JOSH - case analysis on gmap, (eliminator) given function for 
+  cases, produces B (no induction)*)
+  Local Definition gmap_dep_ne_case {A P B} (t : gmap_dep_ne A P)
+    (f : gmap_dep A P~0 → option (P 1 * A) → gmap_dep A P~1 → B) : B :=
+  match t with
+  | GNode001 r => f GEmpty None (GNodes r)
+  | GNode010 p x => f GEmpty (Some (p,x)) GEmpty
+  | GNode011 p x r => f GEmpty (Some (p,x)) (GNodes r)
+  | GNode100 l => f (GNodes l) None GEmpty
+  | GNode101 l r => f (GNodes l) None (GNodes r)
+  | GNode110 l p x => f (GNodes l) (Some (p,x)) GEmpty
+  | GNode111 l p x r => f (GNodes l) (Some (p,x)) (GNodes r)
+  end.
+
+
+Local Definition gmap_dep_omap_aux {A B P}
+    (go : gmap_dep_ne A P → gmap_dep B P) (tm : gmap_dep A P) : gmap_dep B P :=
+  match tm with GEmpty => GEmpty | GNodes t' => go t' end.
+
+(*START*)
+Local Definition gmap_dep_ne_omap {A B} (f : positive -> A → option B) :
+    ∀ {P}, gmap_dep_ne A P → gmap_dep B P :=
+  fix go {P} t :=
+    gmap_dep_ne_case t $ λ ml mx mr,
+      GNode (gmap_dep_omap_aux go ml) ('(p,x) ← mx; (p,.) <$> f x)
+            (gmap_dep_omap_aux go mr).
+
+
+Local Definition gmap_merge_aux {A B C P}
+    (go : gmap_dep_ne A P → gmap_dep_ne B P → gmap_dep C P)
+    (f : positive -> option A → option B → option C)
+    (mt1 : gmap_dep A P) (mt2 : gmap_dep B P) : gmap_dep C P :=
+  match mt1, mt2 with
+  | GEmpty, GEmpty => GEmpty
+  | GNodes t1', GEmpty => gmap_dep_ne_omap (λ x, f (Some x) None) t1'
+  | GEmpty, GNodes t2' => gmap_dep_ne_omap (λ x, f None (Some x)) t2'
+  | GNodes t1', GNodes t2' => go t1' t2'
+  end.
+
+Local Definition diag_None' {A B C} {P : Prop}
+    (f : option A → option B → option C)
+    (mx : option (P * A)) (my : option (P * B)) : option (P * C) :=
+  match mx, my with
+  | None, None => None
+  | Some (p,x), None => (p,.) <$> f (Some x) None
+  | None, Some (p,y) => (p,.) <$> f None (Some y)
+  | Some (p,x), Some (_,y) => (p,.) <$> f (Some x) (Some y)
+  end.
+
+
+Local Definition gmap_dep_ne_merge {A B C} (f : positive -> option A → option B → option C) :
+    ∀ {P}, gmap_dep_ne A P → gmap_dep_ne B P → gmap_dep C P :=
+  fix go {P} t1 t2 {struct t1} :=
+    gmap_dep_ne_case t1 $ λ ml1 mx1 mr1,
+      gmap_dep_ne_case t2 $ λ ml2 mx2 mr2,
+        GNode (gmap_merge_aux go f ml1 ml2) (diag_None' f mx1 mx2)
+              (gmap_merge_aux go f mr1 mr2).
+Local Definition gmap_dep_merge {A B C P} (f : positive -> option A → option B → option C) :
+    gmap_dep A P → gmap_dep B P → gmap_dep C P :=
+  gmap_merge_aux (gmap_dep_ne_merge f) f.
+Global Instance gmap_merge `{Countable K} : Merge (gmap K) :=
+  λ {A B C} f '(GMap mt1) '(GMap mt2), GMap $ gmap_dep_merge f mt1 mt2.
+Print gmap_merge.
+Print gmap_dep_merge.
+
+
+Print gmap_key.
+Print gmap_dep_ne.
+Print UnionWith.
+Search UnionWith gmap.
+Search Merge gmap.
+Search Union gmap.
+Print Union.
+
+Definition gmap_union2 {K: Type} `{Countable K}
+  {A B: Type} (f: K -> A -> A -> option A) (g1 g2: gmap K A) : gmap K A :=
+  GMap _.
+
+
+Parameter union: (key -> a -> a -> option a) -> t a -> t a -> t a.
+
+  Parameter merge: (key -> option a -> option b -> option c) ->
+  t a -> t b -> t c.
+
+Print gmap.
+
+Local Definition gmap_merge_aux {A B C P}
+    (go : gmap_dep_ne A P → gmap_dep_ne B P → gmap_dep C P)
+    (f : positive -> option A → option B → option C)
+    (mt1 : gmap_dep A P) (mt2 : gmap_dep B P) : gmap_dep C P :=
+  match mt1, mt2 with
+  | GEmpty, GEmpty => GEmpty
+  | GNodes t1', GEmpty => gmap_dep_ne_omap (λ x, f (Some x) None) t1'
+  | GEmpty, GNodes t2' => gmap_dep_ne_omap (λ x, f None (Some x)) t2'
+  | GNodes t1', GNodes t2' => go t1' t2'
+  end.
+
+  *)
+
 Module Type S.
 
 Parameter key: Type.
@@ -17,6 +141,173 @@ Variable acc: Type.
 
 Parameter empty: t a.
 Parameter is_empty: t a -> bool.
+Parameter mem: key -> t a -> bool.
+Parameter add: key -> a -> t a -> t a.
+Parameter singleton: key -> a -> t a.
+Parameter remove: key -> t a -> t a.
+Parameter merge: (key -> option a -> option b -> option c) ->
+  t a -> t b -> t c.
+Parameter union: (key -> a -> a -> option a) -> t a -> t a -> t a.
+(*TODO: to OCaml int? and do we need in general?*)
+(*Parameter compare: (a -> a -> Z) -> t a -> t a -> Z.*)
+(*START*)
+(*Parameter equal: (a -> a -> bool) -> t a -> t a -> bool.*)
+Parameter equal: EqDecision a -> t a -> t a -> bool.
+(*Parameter iter: (key -> a -> unit) -> t a -> unit.
+Parameter fold: (key -> a -> b -> b) -> t a -> b -> b.
+Parameter for_all: (key -> a -> bool) -> t a -> bool.
+(*Note: reserved keyword*)
+Parameter exists_: (key -> a -> bool) -> t a -> bool.
+Parameter filter: (key -> a -> bool) -> t a -> t a.
+Parameter partition: (key -> a -> bool) -> t a -> (t a * t a).
+Parameter cardinal: t a -> positive.
+Parameter bindings: t a -> list (key * a).
+(*NOTE: need to change - throws exception*)
+Parameter min_binding: t a -> (key * a).
+Parameter max_binding: t a -> (key * a).
+Parameter choose: t a -> (key * a).
+Parameter split: key -> t a -> t a * option a * t a.
+Parameter find: key -> t a -> a.
+Parameter map: (a -> b) -> t a -> t b.
+Parameter mapi: (key -> a -> b) -> t a -> t b.
+
+Parameter change: (option a -> option a) -> key -> t a -> t a.
+Parameter inter: (key -> a -> b -> option c) -> t a -> t b -> t c.
+Parameter diff: (key -> a -> b -> option a) -> t a -> t b -> t a.
+Parameter submap: (key -> a -> b -> bool) -> t a -> t b -> bool.
+Parameter disjoint: (key -> a -> b -> bool) -> t a -> t b -> bool.
+Parameter set_union: t a -> t a -> t a.
+Parameter set_inter: t a -> t b -> t a.
+Parameter set_diff: t a -> t b -> t a.
+Parameter set_submap: t a -> t b -> bool.
+Parameter set_disjoint: t a -> t b -> bool.
+Parameter set_compare: t a -> t b -> Z.
+Parameter set_equal: t a -> t b -> bool.
+Parameter find_def: a -> key -> t a -> a.
+Parameter find_opt: key -> t a -> option a.
+(*TODO: handle exceptions and error handling*)
+(*Parameter find_exn: exn -> key -> t a -> a.*)
+Parameter map_filter: (a -> option b) -> t a -> t b.
+Parameter mapi_filter: (key -> a -> option b) -> t a -> t b.
+Parameter mapi_fold: (key -> a -> acc -> acc * b) -> t a -> acc -> acc * t b.
+Parameter mapi_filter_fold: (key -> a -> acc-> acc * option b) -> t a -> acc -> acc * t b.
+Parameter fold_left: (b -> key -> a -> b) -> b -> t a -> b.
+Parameter fold2_inter: (key -> a -> b -> c -> c) -> t a -> t b -> c ->c.
+Parameter fold2_union: (key -> option a -> option b -> c -> c) -> t a -> t b -> c -> c.
+Parameter translate: (key -> key) -> t a -> t a.
+(*Parameter add_new: exn -> key -> a -> t a -> t a.*)
+(*Parameter replace: exn -> key -> a -> t a -> t a*)
+Parameter keys: t a -> list key.
+Parameter values: t a -> list a.
+Parameter of_list: list (key * a) -> t a.
+Parameter contains: t a -> key -> bool.
+Parameter domain: t a -> t unit.
+Parameter subdomain: (key -> a -> bool) -> t a -> t unit.
+(*TODO: OCaml int?*)
+Parameter is_num_elt: positive -> t a -> bool.
+Parameter enumeration: Type -> Type.
+Parameter val_enum: enumeration a -> option (key * a).
+Parameter start_enum: t a -> enumeration a.
+Parameter next_enum: enumeration a -> enumeration a.
+Parameter start_ge_enum: key -> t a -> enumeration a.
+Parameter next_ge_enum: key -> enumeration a -> enumeration a.*)
+
+End Types.
+
+End S.
+
+(*Different from theirs: use hashed type instead of
+  ordered*)
+Module Type TaggedType.
+Parameter t : Type.
+Parameter tag: t -> positive.
+(*NOTE: we need a form of decidable equality: this
+  is different from the OCaml implementation, which takes in
+  an ordered type*)
+Parameter eq_dec : EqDecision t. 
+End TaggedType.
+
+Module Make (T: TaggedType) <: S.
+
+Definition key := T.t.
+
+(*Union, merge, etc need to know key for function, so 
+  we store it as well. We could modify gmap, maybe we will
+  do that later*)
+Definition t (A: Type) : Type := gmap positive (key * A).
+
+Section Types.
+
+Variable a: Type.
+Variable b: Type.
+Variable c: Type.
+Variable acc: Type.
+
+Definition empty: t a := gmap_empty.
+
+Definition is_empty (m: t a): bool :=
+  match (gmap_car m) with
+  | GEmpty => true
+  | _ => false
+  end.
+
+Definition mem (k: key) (m: t a) : bool :=
+  match m !! (T.tag k) with
+  | None => false
+  | Some _ => true
+  end.
+
+Definition add (k: key) (v: a) (m: t a) : t a :=
+  <[T.tag k:=(k, v)]> m.
+
+Definition singleton (k: key) (v: a) : t a :=
+  {[T.tag k:=(k, v)]}.
+
+Definition remove (k: key) (m: t a) : t a :=
+  delete (T.tag k) m.
+
+(*The gmap merge function does not use the key, so we need
+  a bit of an awkward encoding*)
+
+(*TODO: clean up*)
+(*Need true polymorphism here for union*)
+Definition merge {a b c: Type} (f: key -> option a -> option b -> option c)
+  (m1: t a) (m2: t b) : t c := @merge _ (gmap_merge) _ _ _
+    (*NOTE: k1 and k2 are always the same by the correctness of
+      the merge operation and our invariants*)
+    (fun (x: option (key * a)) (y: option (key * b)) =>
+      match x with
+      | Some (k1, v1) => option_map (pair k1) 
+                          (f k1 (Some v1) (option_map snd y))
+      | None => 
+        match y with
+        | Some (k2, v2) => option_map (pair k2)
+                              (f k2 None (Some v2))
+        | _ => None
+        end
+      end
+    ) m1 m2.
+
+(*Follow OCaml spec of union in terms of merge*)
+Definition union (f: key -> a -> a -> option a) (m1: t a) (m2: t a):
+  t a := 
+  merge (fun k v1 v2 =>
+    match v1, v2 with
+    | None, None => None
+    | Some v1, None => Some v1
+    | None, Some v2 => Some v2
+    | Some v1, Some v2 => f k v1 v2
+    end) m1 m2.
+
+
+Definition equal (eq: EqDecision a) (m1: t a) (m2: t a) : bool :=
+  if (gmap_eq_dec (@prod_eq_dec _ T.eq_dec _ eq)) m1 m2 
+  then true else false.
+
+End Types.
+End Make.
+
+(*Parameter is_empty: t a -> bool.
 Parameter mem: key -> t a -> bool.
 Parameter add: key -> a -> t a -> t a.
 Parameter singleton: key -> a -> t a.
@@ -88,4 +379,7 @@ Parameter next_ge_enum: key -> enumeration a -> enumeration a.
 
 End Types.
 
-End S.
+
+End Make.
+
+Parameter compare: *)
