extract/Extract.v
@@ -1,17 +1,31 @@
 From Src.core Require Import Ident Ty.
+From Src.util Require Import Extmap.
+From stdpp Require Import gmap.
 From Coq Require Extraction.
+
+Require Import Coq.extraction.ExtrOcamlBasic.
 
 Unset Extraction KeepSingleton.
 (*Of course TODO*)
 Extract Constant position => "int".
-Extract Inductive bool => "bool" [ "true" "false" ].
+(*Extract Inductive bool => "bool" [ "true" "false" ].
 Extract Inductive list => "list" [ "[]" "(::)" ].
 Extract Inductive option => "option" [ "None" "Some" ].
 Extract Inductive unit => "unit" [ "()" ].
+Extract Inductive prod => "(*)"  [ "(,)" ].*)
+Extract Inlined Constant Datatypes.fst => "fst".
+Extract Inlined Constant Datatypes.snd => "snd".
 Extraction Inline ty_build.
 Extraction Inline ty_build'.
 Extraction Inline ty_build_simpl.
 Extraction Inline ty_build_simpl'.
-Separate Extraction Ty.ty Ty.ty_v_map Ident.
+Extraction Inline Decision RelDecision.
+(*TODO: why aren't these extracted?*)
+(*Extraction "Datatypes.ml" Datatypes.id.
+Separate Extraction gmap.gmap gmap.gmap_merge.*)
+Separate Extraction (*gmap.gmap gmap.gmap_empty*) 
+  Extmap Ty.ty Ty.ty_v_map Ident.
+(*Separate Extraction Extmap.
+Separate Extraction Ty.ty Ty.ty_v_map Ident.*)
 
 (*Recursive Extraction Library Ty.*)
